feat: HasAll in headers

src/Std/Internal/Http/Data/Header/Map.lean
@@ -6,10 +6,7 @@ Authors: Sofia Rodrigues
 module
 
 prelude
-public import Init.Data.Slice
-public import Init.Data.String
 public import Std.Data.HashMap
-public import Std.Data.HashSet
 public import Std.Internal.Http.Data.Header.Name
 public import Std.Internal.Http.Internal
 
@@ -29,7 +26,6 @@ open Std Internal
 
 set_option linter.all true
 
-
 /--
 A structure for managing HTTP headers as key-value pairs.
 -/
@@ -38,19 +34,43 @@ structure Headers where
   The internal hashmap that stores all the data.
   -/
   data : HashMap HeaderName (Array HeaderValue)
+  deriving Repr, Inhabited
 
-deriving Repr, Inhabited
+instance : Membership HeaderName Headers where
+  mem h s := s ∈ h.data
+
+instance (name : HeaderName) (h : Headers) : Decidable (name ∈ h) :=
+  inferInstanceAs (Decidable (name ∈ h.data))
 
 namespace Headers
 
 /--
+Proposition that a string corresponds to a valid header name present in the headers.
+-/
+abbrev In (s : String) (h : Headers) : Prop :=
+  match HeaderName.ofString? s with
+  | some name => name ∈ h
+  | none => False
+
+instance {s : String} {h : Headers} : Decidable (In s h) := by
+  unfold In
+  cases headerName : HeaderName.ofString? s
+  all_goals exact inferInstance
+
+/--
 Retrieves the `HeaderValue` for the given key.
-Returns `none` if the header is absent.
 -/
 @[inline]
-def get (headers : Headers) (name : HeaderName) : Option HeaderValue :=
-  headers.data.get? name
-  |>.map (.joinCommaSep)
+def get (headers : Headers) (name : HeaderName) (h : name ∈ headers) : HeaderValue :=
+  headers.data.get name h
+  |> HeaderValue.joinCommaSep
+
+/--
+Retrieves all `HeaderValue` entries for the given key.
+-/
+@[inline]
+def getAll (headers : Headers) (name : HeaderName) (h : name ∈ headers) : Array HeaderValue :=
+  headers.data.get name h
 
 /--
 Retrieves all `HeaderValue` entries for the given key.
@@ -58,7 +78,21 @@ Returns `none` if the header is absent.
 -/
 @[inline]
 def getAll? (headers : Headers) (name : HeaderName) : Option (Array HeaderValue) :=
-  headers.data.get? name
+  if h : name ∈ headers then
+    some (headers.getAll name h)
+  else
+    none
+
+/--
+Retrieves the `HeaderValue` for the given key.
+Returns `none` if the header is absent.
+-/
+@[inline]
+def get? (headers : Headers) (name : HeaderName) : Option HeaderValue :=
+  if h : name ∈ headers then
+    some (headers.get name h)
+  else
+    none
 
 /--
 Checks if the entry is present in the `Headers`.
@@ -78,27 +112,25 @@ def getLast? (headers : Headers) (name : HeaderName) : Option HeaderValue :=
   headers.data.get? name
   |>.bind (fun x => x[x.size - 1]?)
 
-
 /--
 Like `get?`, but returns a default value if absent.
 -/
 @[inline]
 def getD (headers : Headers) (name : HeaderName) (d : HeaderValue) : HeaderValue :=
-  headers.get name |>.getD d
+  headers.get? name |>.getD d
 
 /--
 Like `get?`, but panics if absent.
 -/
 @[inline]
 def get! (headers : Headers) (name : HeaderName) : HeaderValue :=
-  headers.get name |>.get!
+  headers.get? name |>.get!
 
 /--
 Inserts a new key-value pair into the headers.
 -/
 @[inline]
 def insert (headers : Headers) (key : HeaderName) (value : HeaderValue) : Headers :=
-
   if let some headerValue := headers.data.get? key then
     { data := headers.data.insert key (headerValue.push value) }
   else
@@ -169,4 +201,92 @@ instance : ToString Headers where
 instance : Encode .v11 Headers where
   encode buffer := buffer.writeString ∘ toString
 
+instance : EmptyCollection Headers := ⟨Headers.empty⟩
+
+instance : Singleton (HeaderName × HeaderValue) Headers := ⟨fun ⟨a, b⟩ => (∅ : Headers).insert a b⟩
+
+instance : Insert (HeaderName × HeaderValue) Headers := ⟨fun ⟨a, b⟩ s => s.insert a b⟩
+
+instance : Union Headers := ⟨merge⟩
+
+/--
+Proposition that all strings in a list are present in the headers.
+-/
+inductive HasAll : (h : Headers) → (l : List String) → Prop where
+  /--
+  The empty list is trivially present in any headers.
+  -/
+  | nil : HasAll h []
+
+  /--
+  If a string is in headers and the rest of the list satisfies HasAll,
+  then the whole list satisfies HasAll.
+  -/
+  | cons (member : In s h) (tail : HasAll h rest) : HasAll h (s :: rest)
+
+namespace HasAll
+
+theorem in_of_hasall (name : String) (inList : name ∈ list) (hasAll : HasAll headers list) : In name headers :=
+  match hasAll with
+  | .nil => by contradiction
+  | @HasAll.cons s _ _ member tail =>
+    if eq : s = name then
+      eq ▸ member
+    else
+      in_of_hasall name (List.mem_of_ne_of_mem (Ne.intro (fun x => eq x.symm)) inList) tail
+
+theorem in_implies_valid (h : In name headers) : isValidHeaderName name :=
+  if h₀ : isValidHeaderName name then h₀ else by
+    unfold In HeaderName.ofString? at h
+    simp [h₀] at h
+
+theorem mem_implies_valid (name : String) (inList : name ∈ list) (hasAll : HasAll headers list) : isValidHeaderName name :=
+  in_implies_valid (in_of_hasall name inList hasAll)
+
+theorem in_implies_mem (h : In nn headers) : ∃p : (isValidHeaderName nn), HeaderName.mk nn p ∈ headers := by
+  simp [In, HeaderName.ofString?] at h
+  if h2 : isValidHeaderName nn then
+    simp [eq_true h2] at h
+    exact ⟨_, h⟩
+  else
+    simp [eq_false h2] at h
+
+theorem tail (hasAll : HasAll headers (h :: t)) : HasAll headers t := by
+  cases hasAll with
+  | cons _ tail => exact tail
+
+theorem head : (hasAll : HasAll headers (h :: t)) → In h headers
+  | cons member _ => member
+
+/--
+Decision procedure for `HasAll`.
+-/
+def decidable : Decidable (HasAll h l) :=
+  match l with
+  | [] => isTrue HasAll.nil
+  | head :: tail =>
+    if headMember : In head h then
+      match @decidable h tail with
+      | isTrue tailHasAll => Decidable.isTrue (HasAll.cons headMember tailHasAll)
+      | isFalse notTailHasAll => Decidable.isFalse fun hasAll => notTailHasAll hasAll.tail
+    else
+      Decidable.isFalse fun hasAll => headMember hasAll.head
+
+/--
+Gets the value of a header by name.
+-/
+def get (hasAll : HasAll headers l) (name : String) (h : (name ∈ l) := by get_elem_tactic) : HeaderValue :=
+  let h2 := in_implies_mem (in_of_hasall name h hasAll)
+  headers.get (HeaderName.mk name h2.choose) h2.choose_spec
+
+/--
+Gets all values of a header by name.
+-/
+def getAll (hasAll : HasAll headers l) (name : String) (h : (name ∈ l) := by get_elem_tactic) : Array HeaderValue :=
+  let h2 := in_implies_mem (in_of_hasall name h hasAll)
+  headers.getAll (HeaderName.mk name h2.choose) h2.choose_spec
+
+instance : Decidable (HasAll h l) := decidable
+
+end HasAll
 end Std.Http.Headers
